Classes/Except.v
@@ -3,14 +3,14 @@ Require Import Classes.Applicative.
 Require Import Classes.Monad.
 
 Class Except (M : Type -> Type) `{Monad M} := {
-  throw    : M unit;
-  trycatch : M unit -> M unit -> M unit;
-  bind_fail : forall (f : unit -> M unit), bindM throw f = throw;
-  trycatch_throw_left : forall (x : M unit), 
+  throw    : forall {A}, M A;
+  trycatch : forall {A}, M A -> M A -> M A;
+  bind_fail : forall {A} (f : unit -> M A), bindM throw f = throw;
+  trycatch_throw_left : forall {A} (x : M A), 
     trycatch throw x = x;
-  trycatch_throw_right : forall (x : M unit),
+  trycatch_throw_right : forall {A} (x : M A),
     trycatch x throw = x;
-  trycatch_pure : forall x h, trycatch (pure x) h = pure x;
+  trycatch_pure : forall {A} x h, trycatch (pure x) h = pure (A:=A) x;
 }.
 
 Hint Rewrite @trycatch_throw_left @trycatch_throw_right 
