Instances/IsNat/Nat.v
@@ -9,27 +9,27 @@ Require Import Classes.Applicative.
 
 Definition ensure_nat (v : cvalue) : ConcreteState nat :=
   match v with
-  | VNat x => pure_maybeT _ (pure x)
-  | _ => pure None 
+  | VNat x => liftT (pure x)
+  | _ => liftT (pure None)
   end.
 
 Definition extract_natM (n : nat) : ConcreteState nat :=
-  pure_maybeT _ (pure n).
+  liftT (pure n).
 
 Definition plusM (n m : nat) : ConcreteState nat := 
-  pure_maybeT _ (pure (plus n m)).
+  liftT (pure (plus n m)).
 
 Definition multM (n m : nat) : ConcreteState nat := 
-  pure_maybeT _ (pure (mult n m)).
+  liftT (pure (mult n m)).
 
 Definition eqbM (n m : nat) : ConcreteState bool := 
-  pure_maybeT _ (pure (Nat.eqb n m)).
+  liftT (pure (Nat.eqb n m)).
 
 Definition lebM (n m : nat) : ConcreteState bool := 
-  pure_maybeT _ (pure (Nat.leb n m)).
+  liftT (pure (Nat.leb n m)).
 
 Definition build_natural (n : nat) : ConcreteState cvalue := 
-  pure_maybeT _ (pure (VNat n)).
+  liftT (pure (VNat n)).
 
 Global Instance nat_numerical : IsNat ConcreteState cvalue bool nat :=
 {
