Instances/Store/ConcreteStore.v
@@ -10,40 +10,73 @@ Require Import Classes.Monad.
 Require Import Classes.Applicative.
 Require Import Classes.Functor.
 
-Section store_stateT. 
-  Context (M : Type -> Type) `{Monad M}.
+Section store_stateT_concrete. 
+  Context (M : Type -> Type) `{Monad M, Applicative M}.
 
-  Definition stateT_get (S : Type) := fun s : S => pure(s, s).
+  Definition stateT_get (S : Type) := fun s : S => pure (s, s).
 
-  Definition stateT_put (S : Type) := fun s : S => fun _ : S => pure(tt, s).
+  Definition stateT_put (S : Type) := fun s : S => fun _ : S => pure (tt, s).
+
+  Definition retrieve_concrete (x : string) : StateT store M cvalue :=
+    fun s : store => pure(s x, s).
+
+  Definition update_concrete (x : string) (v : cvalue) : StateT store M store :=
+    fun s : store => let s' := t_update s x v in pure(s', s').
 
   Global Instance store_stateT (S : Type) : 
-  Store S (StateT S M) (inst:=monad_stateT S) :=
+  Store store (StateT store M) cvalue :=
   {
-    get := @stateT_get S;
-    put := @stateT_put S;
+    get := stateT_get store;
+    put := stateT_put store;
+    retrieve := retrieve_concrete;
+    update := update_concrete;
   }.
-End store_stateT.
+End store_stateT_concrete.
+
+Section store_stateT_abstract.
+  Context (M : Type -> Type) `{Monad M, Applicative M}.
+
+  Definition get_abstract (S : Type) := fun s : S => pure (s, s).
+  Definition put_abstract (S : Type) := fun s : S => fun _ : S => pure (tt, s).
+  Definition retrieve_abstract (x : string) : StateT abstract_store M avalue :=
+    fun s : abstract_store => pure (s x, s).
+  Definition update_abstract (x : string) (v : avalue) : 
+    StateT abstract_store M abstract_store :=
+    fun s : abstract_store => let s' := t_update s x v in pure(s', s').
+
+  Global Instance store_stateT_abstract (S : Type) : 
+    Store abstract_store (StateT abstract_store M) avalue :=
+  {
+    get := get_abstract abstract_store;
+    put := put_abstract abstract_store;
+    retrieve := retrieve_abstract;
+    update := update_abstract;
+  }.
+End store_stateT_abstract.
+
 
 Section store_maybeT.
-  Context {M : Type -> Type} `{inst : Monad M}.
+  Context {M : Type -> Type} `{inst : Monad M} {V : Type}.
 
-  Global Instance store_maybeT (S : Type) `{Store S M} :
-  Store S (MaybeT M) :=
+  Global Instance store_maybeT (S : Type) `{Store S M V} :
+  Store S (MaybeT M) V :=
   {
-    get := fmap Just get;
+    get := liftT get;
     put := fun s => put s ;; pure (Just tt);
+    retrieve := fun x : string => liftT (retrieve x);
+    update := fun x v => liftT (update x v);
   }.
-
 End store_maybeT.
 
 Section store_maybeAT.
-  Context {M : Type -> Type} `{inst : Monad M}.
+  Context {M : Type -> Type} `{inst : Monad M} {V : Type}.
 
-  Global Instance store_maybeAT (S : Type) `{Store S M} :
-  Store S (MaybeAT M) :=
+  Global Instance store_maybeAT (S : Type) `{Store S M V} :
+  Store S (MaybeAT M) V :=
   {
     get := fmap JustA get;
     put := fun s => put s ;; pure (JustA tt);
+    retrieve := fun x => liftT (retrieve x);
+    update := fun x v => liftT (update x v);
   }.
 End store_maybeAT.
