Types/Stores.v
@@ -3,3 +3,10 @@ Require Import Language.Statements.
 
 Definition abstract_store := total_map avalue.
 Definition store := total_map cvalue.
+
+Definition abstract_update (s : abstract_store) (x : string) (v : avalue) :
+  abstract_store := t_update s x v.
+
+Definition concrete_update (s : store) (x : string) (v : cvalue) :
+  store := t_update s x v.
+
